src/opt/ReorderStep.v
@@ -87,12 +87,12 @@ Proof.
 Qed.
 
 Lemma future_is_racy
-      lc1 mem1 mem1' loc ord
+      lc1 mem1 mem1' loc to ord
       (WF: Local.wf lc1 mem1)
       (MEM: Memory.closed mem1)
       (FUTURE: Memory.future_weak mem1 mem1')
-      (STEP: Local.is_racy lc1 mem1 loc ord):
-  <<STEP: Local.is_racy lc1 mem1' loc ord>>.
+      (STEP: Local.is_racy lc1 mem1 loc to ord):
+  <<STEP: Local.is_racy lc1 mem1' loc to ord>>.
 Proof.
   inv STEP.
   exploit Memory.future_weak_get1; eauto. i. des.
@@ -102,36 +102,36 @@ Proof.
 Qed.
 
 Lemma future_racy_read_step
-      lc1 mem1 mem1' loc val ord
+      lc1 mem1 mem1' loc to val ord
       (WF: Local.wf lc1 mem1)
       (MEM: Memory.closed mem1)
       (FUTURE: Memory.future_weak mem1 mem1')
-      (STEP: Local.racy_read_step lc1 mem1 loc val ord):
-  <<STEP: Local.racy_read_step lc1 mem1' loc val ord>>.
+      (STEP: Local.racy_read_step lc1 mem1 loc to val ord):
+  <<STEP: Local.racy_read_step lc1 mem1' loc to val ord>>.
 Proof.
   inv STEP.
   exploit future_is_racy; eauto.
 Qed.
 
 Lemma future_racy_write_step
-      lc1 mem1 mem1' loc ord
+      lc1 mem1 mem1' loc to ord
       (WF: Local.wf lc1 mem1)
       (MEM: Memory.closed mem1)
       (FUTURE: Memory.future_weak mem1 mem1')
-      (STEP: Local.racy_write_step lc1 mem1 loc ord):
-  <<STEP: Local.racy_write_step lc1 mem1' loc ord>>.
+      (STEP: Local.racy_write_step lc1 mem1 loc to ord):
+  <<STEP: Local.racy_write_step lc1 mem1' loc to ord>>.
 Proof.
   inv STEP.
   exploit future_is_racy; eauto.
 Qed.
 
 Lemma future_racy_update_step
-      lc1 mem1 mem1' loc ordr ordw
+      lc1 mem1 mem1' loc to ordr ordw
       (WF: Local.wf lc1 mem1)
       (MEM: Memory.closed mem1)
       (FUTURE: Memory.future_weak mem1 mem1')
-      (STEP: Local.racy_update_step lc1 mem1 loc ordr ordw):
-  <<STEP: Local.racy_update_step lc1 mem1' loc ordr ordw>>.
+      (STEP: Local.racy_update_step lc1 mem1 loc to ordr ordw):
+  <<STEP: Local.racy_update_step lc1 mem1' loc to ordr ordw>>.
 Proof.
   inv STEP.
   - econs 1; eauto.
@@ -373,12 +373,12 @@ Qed.
 
 Lemma reorder_read_is_racy
       loc1 ts1 val1 released1 ord1
-      loc2 ord2
+      loc2 to2 ord2
       lc0 mem0
       lc1
       (STEP1: Local.read_step lc0 mem0 loc1 ts1 val1 released1 ord1 lc1)
-      (STEP2: Local.is_racy lc1 mem0 loc2 ord2):
-  <<STEP1: Local.is_racy lc0 mem0 loc2 ord2>>.
+      (STEP2: Local.is_racy lc1 mem0 loc2 to2 ord2):
+  <<STEP1: Local.is_racy lc0 mem0 loc2 to2 ord2>>.
 Proof.
   inv STEP1. inv STEP2. ss.
   econs; try exact GET0; eauto.
@@ -388,12 +388,12 @@ Qed.
 
 Lemma reorder_read_racy_read
       loc1 ts1 val1 released1 ord1
-      loc2 val2 ord2
+      loc2 to2 val2 ord2
       lc0 mem0
       lc1
       (STEP1: Local.read_step lc0 mem0 loc1 ts1 val1 released1 ord1 lc1)
-      (STEP2: Local.racy_read_step lc1 mem0 loc2 val2 ord2):
-  <<STEP1: Local.racy_read_step lc0 mem0 loc2 val2 ord2>>.
+      (STEP2: Local.racy_read_step lc1 mem0 loc2 to2 val2 ord2):
+  <<STEP1: Local.racy_read_step lc0 mem0 loc2 to2 val2 ord2>>.
 Proof.
   inv STEP2.
   exploit reorder_read_is_racy; eauto.
@@ -401,12 +401,12 @@ Qed.
 
 Lemma reorder_read_racy_write
       loc1 ts1 val1 released1 ord1
-      loc2 ord2
+      loc2 to2 ord2
       lc0 mem0
       lc1
       (STEP1: Local.read_step lc0 mem0 loc1 ts1 val1 released1 ord1 lc1)
-      (STEP2: Local.racy_write_step lc1 mem0 loc2 ord2):
-  <<STEP1: Local.racy_write_step lc0 mem0 loc2 ord2>>.
+      (STEP2: Local.racy_write_step lc1 mem0 loc2 to2 ord2):
+  <<STEP1: Local.racy_write_step lc0 mem0 loc2 to2 ord2>>.
 Proof.
   inv STEP2.
   hexploit read_step_promise_consistent; eauto. i.
@@ -606,13 +606,13 @@ Qed.
 
 Lemma reorder_fulfill_is_racy
       loc1 from1 to1 val1 releasedm1 released1 ord1
-      loc2 ord2
+      loc2 to2 ord2
       lc0 sc0 mem0
       lc1 sc1
       (LOC: loc1 <> loc2)
       (STEP1: fulfill_step lc0 sc0 loc1 from1 to1 val1 releasedm1 released1 ord1 lc1 sc1)
-      (STEP2: Local.is_racy lc1 mem0 loc2 ord2):
-  <<STEP1: Local.is_racy lc0 mem0 loc2 ord2>>.
+      (STEP2: Local.is_racy lc1 mem0 loc2 to2 ord2):
+  <<STEP1: Local.is_racy lc0 mem0 loc2 to2 ord2>>.
 Proof.
   inv STEP1. inv STEP2. ss.
   econs; try exact GET; eauto.
@@ -625,13 +625,13 @@ Qed.
 
 Lemma reorder_fulfill_racy_read
       loc1 from1 to1 val1 releasedm1 released1 ord1
-      loc2 val2 ord2
+      loc2 to2 val2 ord2
       lc0 sc0 mem0
       lc1 sc1
       (LOC: loc1 <> loc2)
       (STEP1: fulfill_step lc0 sc0 loc1 from1 to1 val1 releasedm1 released1 ord1 lc1 sc1)
-      (STEP2: Local.racy_read_step lc1 mem0 loc2 val2 ord2):
-  <<STEP1: Local.racy_read_step lc0 mem0 loc2 val2 ord2>>.
+      (STEP2: Local.racy_read_step lc1 mem0 loc2 to2 val2 ord2):
+  <<STEP1: Local.racy_read_step lc0 mem0 loc2 to2 val2 ord2>>.
 Proof.
   inv STEP2.
   exploit reorder_fulfill_is_racy; eauto.
@@ -639,13 +639,13 @@ Qed.
 
 Lemma reorder_fulfill_racy_write
       loc1 from1 to1 val1 releasedm1 released1 ord1
-      loc2 ord2
+      loc2 to2 ord2
       lc0 sc0 mem0
       lc1 sc1
       (LOC: loc1 <> loc2)
       (STEP1: fulfill_step lc0 sc0 loc1 from1 to1 val1 releasedm1 released1 ord1 lc1 sc1)
-      (STEP2: Local.racy_write_step lc1 mem0 loc2 ord2):
-  <<STEP1: Local.racy_write_step lc0 mem0 loc2 ord2>>.
+      (STEP2: Local.racy_write_step lc1 mem0 loc2 to2 ord2):
+  <<STEP1: Local.racy_write_step lc0 mem0 loc2 to2 ord2>>.
 Proof.
   inv STEP2.
   hexploit fulfill_step_promise_consistent; eauto. i.
@@ -1090,15 +1090,15 @@ Qed.
 (** reorder racy read *)
 
 Lemma reorder_is_racy_read
-      loc1 ord1
+      loc1 to1 ord1
       loc2 ts2 val2 released2 ord2
       lc0 mem0
       lc2
       (LOC: loc1 = loc2 -> Ordering.le ord1 Ordering.plain /\ Ordering.le ord2 Ordering.plain)
       (ORD2: Ordering.le ord2 Ordering.relaxed)
-      (STEP1: Local.is_racy lc0 mem0 loc1 ord1)
+      (STEP1: Local.is_racy lc0 mem0 loc1 to1 ord1)
       (STEP2: Local.read_step lc0 mem0 loc2 ts2 val2 released2 ord2 lc2):
-  <<STEP: Local.is_racy lc2 mem0 loc1 ord1>>.
+  <<STEP: Local.is_racy lc2 mem0 loc1 to1 ord1>>.
 Proof.
   inv STEP1. inv STEP2. ss.
   econs; eauto; ss. inv READABLE.
@@ -1113,14 +1113,14 @@ Proof.
 Qed.
 
 Lemma reorder_is_racy_fulfill
-      loc1 ord1
+      loc1 to1 ord1
       loc2 from2 to2 val2 releasedm2 released2 ord2
       lc0 sc0 mem0
       lc2 sc2
       (LOC: loc1 <> loc2)
-      (STEP1: Local.is_racy lc0 mem0 loc1 ord1)
+      (STEP1: Local.is_racy lc0 mem0 loc1 to1 ord1)
       (STEP2: fulfill_step lc0 sc0 loc2 from2 to2 val2 releasedm2 released2 ord2 lc2 sc2):
-  <<STEP: Local.is_racy lc2 mem0 loc1 ord1>>.
+  <<STEP: Local.is_racy lc2 mem0 loc1 to1 ord1>>.
 Proof.
   inv STEP1. inv STEP2.
   econs; eauto; ss.
@@ -1131,7 +1131,7 @@ Proof.
 Qed.
 
 Lemma reorder_is_racy_write
-      loc1 ord1
+      loc1 to1 ord1
       loc2 from2 to2 val2 releasedm2 released2 ord2
       lc0 sc0 mem0
       lc2 sc2 mem2
@@ -1142,9 +1142,9 @@ Lemma reorder_is_racy_write
       (WF0: Local.wf lc0 mem0)
       (SC0: Memory.closed_timemap sc0 mem0)
       (MEM0: Memory.closed mem0)
-      (STEP1: Local.is_racy lc0 mem0 loc1 ord1)
+      (STEP1: Local.is_racy lc0 mem0 loc1 to1 ord1)
       (STEP2: Local.write_step lc0 sc0 mem0 loc2 from2 to2 val2 releasedm2 released2 ord2 lc2 sc2 mem2 kind):
-  <<STEP: Local.is_racy lc2 mem2 loc1 ord1>>.
+  <<STEP: Local.is_racy lc2 mem2 loc1 to1 ord1>>.
 Proof.
   exploit write_promise_fulfill; try exact STEP2; eauto. i. des.
   exploit reorder_is_racy_promise; eauto. i. des.
@@ -1152,7 +1152,7 @@ Proof.
 Qed.
 
 Lemma reorder_is_racy_update
-      loc1 ord1
+      loc1 to1 ord1
       loc2 ts2 val2 released2 ord2
       from3 to3 val3 released3 ord3
       lc0 sc0 mem0
@@ -1164,10 +1164,10 @@ Lemma reorder_is_racy_update
       (WF0: Local.wf lc0 mem0)
       (SC0: Memory.closed_timemap sc0 mem0)
       (MEM0: Memory.closed mem0)
-      (STEP1: Local.is_racy lc0 mem0 loc1 ord1)
+      (STEP1: Local.is_racy lc0 mem0 loc1 to1 ord1)
       (STEP2: Local.read_step lc0 mem0 loc2 ts2 val2 released2 ord2 lc2)
       (STEP3: Local.write_step lc2 sc0 mem0 loc2 from3 to3 val3 released2 released3 ord3 lc3 sc3 mem3 kind):
-  <<STEP: Local.is_racy lc3 mem3 loc1 ord1>>.
+  <<STEP: Local.is_racy lc3 mem3 loc1 to1 ord1>>.
 Proof.
   exploit Local.read_step_future; try exact STEP2; eauto. i. des.
   exploit reorder_is_racy_read; eauto; ss. i. des.
@@ -1175,7 +1175,7 @@ Proof.
 Qed.
 
 Lemma reorder_is_racy_fence
-      loc1 ord1
+      loc1 to1 ord1
       ordr2 ordw2
       lc0 sc0 mem0
       lc2 sc2
@@ -1183,9 +1183,9 @@ Lemma reorder_is_racy_fence
       (ORDW2: Ordering.le ordw2 Ordering.acqrel)
       (WF0: Local.wf lc0 mem0)
       (MEM0: Memory.closed mem0)
-      (STEP1: Local.is_racy lc0 mem0 loc1 ord1)
+      (STEP1: Local.is_racy lc0 mem0 loc1 to1 ord1)
       (STEP2: Local.fence_step lc0 sc0 ordr2 ordw2 lc2 sc2):
-  <<STEP: Local.is_racy lc2 mem0 loc1 ord1>>.
+  <<STEP: Local.is_racy lc2 mem0 loc1 to1 ord1>>.
 Proof.
   inv STEP1. inv STEP2. ss.
   econs; eauto; ss.
@@ -1194,36 +1194,36 @@ Proof.
 Qed.
 
 Lemma reorder_racy_read_read
-      loc1 val1 ord1
+      loc1 to1 val1 ord1
       loc2 ts2 val2 released2 ord2
       lc0 mem0
       lc2
       (LOC: loc1 = loc2 -> Ordering.le ord1 Ordering.plain /\ Ordering.le ord2 Ordering.plain)
       (ORD2: Ordering.le ord2 Ordering.relaxed)
-      (STEP1: Local.racy_read_step lc0 mem0 loc1 val1 ord1)
+      (STEP1: Local.racy_read_step lc0 mem0 loc1 to1 val1 ord1)
       (STEP2: Local.read_step lc0 mem0 loc2 ts2 val2 released2 ord2 lc2):
-  <<STEP: Local.racy_read_step lc2 mem0 loc1 val1 ord1>>.
+  <<STEP: Local.racy_read_step lc2 mem0 loc1 to1 val1 ord1>>.
 Proof.
   inv STEP1.
   exploit reorder_is_racy_read; eauto.
 Qed.
 
 Lemma reorder_racy_read_fulfill
-      loc1 val1 ord1
+      loc1 to1 val1 ord1
       loc2 from2 to2 val2 releasedm2 released2 ord2
       lc0 sc0 mem0
       lc2 sc2
       (LOC: loc1 <> loc2)
-      (STEP1: Local.racy_read_step lc0 mem0 loc1 val1 ord1)
+      (STEP1: Local.racy_read_step lc0 mem0 loc1 to1 val1 ord1)
       (STEP2: fulfill_step lc0 sc0 loc2 from2 to2 val2 releasedm2 released2 ord2 lc2 sc2):
-  <<STEP: Local.racy_read_step lc2 mem0 loc1 val1 ord1>>.
+  <<STEP: Local.racy_read_step lc2 mem0 loc1 to1 val1 ord1>>.
 Proof.
   inv STEP1.
   exploit reorder_is_racy_fulfill; eauto.
 Qed.
 
 Lemma reorder_racy_read_write
-      loc1 val1 ord1
+      loc1 to1 val1 ord1
       loc2 from2 to2 val2 releasedm2 released2 ord2
       lc0 sc0 mem0
       lc2 sc2 mem2
@@ -1234,9 +1234,9 @@ Lemma reorder_racy_read_write
       (WF0: Local.wf lc0 mem0)
       (SC0: Memory.closed_timemap sc0 mem0)
       (MEM0: Memory.closed mem0)
-      (STEP1: Local.racy_read_step lc0 mem0 loc1 val1 ord1)
+      (STEP1: Local.racy_read_step lc0 mem0 loc1 to1 val1 ord1)
       (STEP2: Local.write_step lc0 sc0 mem0 loc2 from2 to2 val2 releasedm2 released2 ord2 lc2 sc2 mem2 kind):
-  <<STEP: Local.racy_read_step lc2 mem2 loc1 val1 ord1>>.
+  <<STEP: Local.racy_read_step lc2 mem2 loc1 to1 val1 ord1>>.
 Proof.
   exploit write_promise_fulfill; try exact STEP2; eauto. i. des.
   exploit reorder_racy_read_promise; eauto. i. des.
@@ -1244,7 +1244,7 @@ Proof.
 Qed.
 
 Lemma reorder_racy_read_update
-      loc1 val1 ord1
+      loc1 to1 val1 ord1
       loc2 ts2 val2 released2 ord2
       from3 to3 val3 released3 ord3
       lc0 sc0 mem0
@@ -1256,10 +1256,10 @@ Lemma reorder_racy_read_update
       (WF0: Local.wf lc0 mem0)
       (SC0: Memory.closed_timemap sc0 mem0)
       (MEM0: Memory.closed mem0)
-      (STEP1: Local.racy_read_step lc0 mem0 loc1 val1 ord1)
+      (STEP1: Local.racy_read_step lc0 mem0 loc1 to1 val1 ord1)
       (STEP2: Local.read_step lc0 mem0 loc2 ts2 val2 released2 ord2 lc2)
       (STEP3: Local.write_step lc2 sc0 mem0 loc2 from3 to3 val3 released2 released3 ord3 lc3 sc3 mem3 kind):
-  <<STEP: Local.racy_read_step lc3 mem3 loc1 val1 ord1>>.
+  <<STEP: Local.racy_read_step lc3 mem3 loc1 to1 val1 ord1>>.
 Proof.
   exploit Local.read_step_future; try exact STEP2; eauto. i. des.
   exploit reorder_racy_read_read; eauto; ss. i. des.
@@ -1267,7 +1267,7 @@ Proof.
 Qed.
 
 Lemma reorder_racy_read_fence
-      loc1 val1 ord1
+      loc1 to1 val1 ord1
       ordr2 ordw2
       lc0 sc0 mem0
       lc2 sc2
@@ -1275,9 +1275,9 @@ Lemma reorder_racy_read_fence
       (ORDW2: Ordering.le ordw2 Ordering.acqrel)
       (WF0: Local.wf lc0 mem0)
       (MEM0: Memory.closed mem0)
-      (STEP1: Local.racy_read_step lc0 mem0 loc1 val1 ord1)
+      (STEP1: Local.racy_read_step lc0 mem0 loc1 to1 val1 ord1)
       (STEP2: Local.fence_step lc0 sc0 ordr2 ordw2 lc2 sc2):
-  <<STEP: Local.racy_read_step lc2 mem0 loc1 val1 ord1>>.
+  <<STEP: Local.racy_read_step lc2 mem0 loc1 to1 val1 ord1>>.
 Proof.
   inv STEP1.
   exploit reorder_is_racy_fence; eauto.
