src/opt/SplitAcqCommon.v
@@ -215,15 +215,15 @@ Qed.
 Lemma sim_local_is_racy_acquired
       lc1_src mem1_src
       lc1_tgt mem1_tgt
-      loc
-      (STEP_TGT: Local.is_racy lc1_tgt mem1_tgt loc Ordering.relaxed)
+      loc to
+      (STEP_TGT: Local.is_racy lc1_tgt mem1_tgt loc to Ordering.relaxed)
       (LOCAL1: sim_local SimPromises.bot lc1_src lc1_tgt)
       (MEM1: sim_memory mem1_src mem1_tgt)
       (WF1_SRC: Local.wf lc1_src mem1_src)
       (WF1_TGT: Local.wf lc1_tgt mem1_tgt)
       (MEM1_SRC: Memory.closed mem1_src)
       (MEM1_TGT: Memory.closed mem1_tgt):
-  <<STEP_SRC: Local.is_racy lc1_src mem1_src loc Ordering.acqrel>>.
+  <<STEP_SRC: Local.is_racy lc1_src mem1_src loc to Ordering.acqrel>>.
 Proof.
   exploit sim_local_is_racy; try exact STEP_TGT;
     try exact LOCAL1; try exact MEM1; try refl; eauto. i. des.
@@ -233,15 +233,15 @@ Qed.
 Lemma sim_local_racy_read_acquired
       lc1_src mem1_src
       lc1_tgt mem1_tgt
-      loc val
-      (STEP_TGT: Local.racy_read_step lc1_tgt mem1_tgt loc val Ordering.relaxed)
+      loc to val
+      (STEP_TGT: Local.racy_read_step lc1_tgt mem1_tgt loc to val Ordering.relaxed)
       (LOCAL1: sim_local SimPromises.bot lc1_src lc1_tgt)
       (MEM1: sim_memory mem1_src mem1_tgt)
       (WF1_SRC: Local.wf lc1_src mem1_src)
       (WF1_TGT: Local.wf lc1_tgt mem1_tgt)
       (MEM1_SRC: Memory.closed mem1_src)
       (MEM1_TGT: Memory.closed mem1_tgt):
-  <<STEP_SRC: Local.racy_read_step lc1_src mem1_src loc val Ordering.acqrel>>.
+  <<STEP_SRC: Local.racy_read_step lc1_src mem1_src loc to val Ordering.acqrel>>.
 Proof.
   inv STEP_TGT.
   exploit sim_local_is_racy_acquired; eauto.
@@ -250,15 +250,15 @@ Qed.
 Lemma sim_local_racy_update_acquired
       lc1_src mem1_src
       lc1_tgt mem1_tgt
-      loc ow
-      (STEP_TGT: Local.racy_update_step lc1_tgt mem1_tgt loc Ordering.relaxed ow)
+      loc to ow
+      (STEP_TGT: Local.racy_update_step lc1_tgt mem1_tgt loc to Ordering.relaxed ow)
       (LOCAL1: sim_local SimPromises.bot lc1_src lc1_tgt)
       (MEM1: sim_memory mem1_src mem1_tgt)
       (WF1_SRC: Local.wf lc1_src mem1_src)
       (WF1_TGT: Local.wf lc1_tgt mem1_tgt)
       (MEM1_SRC: Memory.closed mem1_src)
       (MEM1_TGT: Memory.closed mem1_tgt):
-  <<STEP_SRC: Local.racy_update_step lc1_src mem1_src loc Ordering.acqrel ow>>.
+  <<STEP_SRC: Local.racy_update_step lc1_src mem1_src loc to Ordering.acqrel ow>>.
 Proof.
   exploit sim_local_racy_update; try exact STEP_TGT;
     try exact LOCAL1; try exact MEM1; try refl; eauto. i. des.
