src/opt/SplitRelCommon.v
@@ -130,8 +130,8 @@ Qed.
 Lemma sim_local_racy_write_released
       lc1_src sc1_src mem1_src
       lc1_tgt sc1_tgt mem1_tgt
-      loc
-      (STEP_TGT: Local.racy_write_step lc1_tgt mem1_tgt loc Ordering.strong_relaxed)
+      loc to
+      (STEP_TGT: Local.racy_write_step lc1_tgt mem1_tgt loc to Ordering.strong_relaxed)
       (LOCAL1: sim_local SimPromises.bot lc1_src lc1_tgt)
       (SC1: TimeMap.le sc1_src sc1_tgt)
       (MEM1: sim_memory mem1_src mem1_tgt)
@@ -141,7 +141,7 @@ Lemma sim_local_racy_write_released
       (SC1_TGT: Memory.closed_timemap sc1_tgt mem1_tgt)
       (MEM1_SRC: Memory.closed mem1_src)
       (MEM1_TGT: Memory.closed mem1_tgt):
-  <<STEP_SRC: Local.racy_write_step lc1_src mem1_src loc Ordering.acqrel>>.
+  <<STEP_SRC: Local.racy_write_step lc1_src mem1_src loc to Ordering.acqrel>>.
 Proof.
   exploit sim_local_racy_write; try exact STEP_TGT;
     try exact LOCAL1; try exact SC1; try exact MEM1; try refl; eauto. i. des.
@@ -152,8 +152,8 @@ Qed.
 Lemma sim_local_racy_update_released
       lc1_src sc1_src mem1_src
       lc1_tgt sc1_tgt mem1_tgt
-      loc ordr
-      (STEP_TGT: Local.racy_update_step lc1_tgt mem1_tgt loc ordr Ordering.strong_relaxed)
+      loc to ordr
+      (STEP_TGT: Local.racy_update_step lc1_tgt mem1_tgt loc to ordr Ordering.strong_relaxed)
       (LOCAL1: sim_local SimPromises.bot lc1_src lc1_tgt)
       (SC1: TimeMap.le sc1_src sc1_tgt)
       (MEM1: sim_memory mem1_src mem1_tgt)
@@ -163,7 +163,7 @@ Lemma sim_local_racy_update_released
       (SC1_TGT: Memory.closed_timemap sc1_tgt mem1_tgt)
       (MEM1_SRC: Memory.closed mem1_src)
       (MEM1_TGT: Memory.closed mem1_tgt):
-  <<STEP_SRC: Local.racy_update_step lc1_src mem1_src loc ordr Ordering.acqrel>>.
+  <<STEP_SRC: Local.racy_update_step lc1_src mem1_src loc to ordr Ordering.acqrel>>.
 Proof.
   exploit sim_local_racy_update; try exact STEP_TGT;
     try exact LOCAL1; try exact SC1; try exact MEM1; try refl; eauto. i. des.
